@prefix rdf: <http://www.w3.org/1999/02/22-rdf-syntax-ns#> .
@prefix : <http://www.spacerdf.org/schema.xml#> .
@prefix dc: <http://purl.org/dc/elements/1.1/> .
@prefix rdfs: <http://www.w3.org/2000/01/rdf-schema#> .
@prefix foaf: <http://xmlns.com/foaf/0.1/> .
@prefix owl: <http://www.w3.org/2002/07/owl#> .
@prefix xsd: <http://www.w3.org/2001/XMLSchema#> .

dc:title
    a owl:AnnotationProperty .

<http://www.spacerdf.org/schema.xml#>
    dc:title "SpaceRDF Vocabulary" ;
    a owl:Ontology ;
    rdfs:comment "RDF vocabulary for describing hackerspaces and related concepts" ;
    owl:imports <http://xmlns.com/foaf/0.1/> .

:Space
    a owl:Class ;
    rdfs:comment "A space is a physical place, where people can meet and work on their projects. Currently, no effort is made to seperate the physical space from the group of people that use it or any formal organisation structure." ;
    rdfs:isDefinedBy <http://www.spacerdf.org/schema.xml> ;
    rdfs:subClassOf foaf:Group ;
    owl:disjointWith :State .

:SpaceAPIDocument
    a owl:Class ;
    rdfs:comment "A SpaceAPI JSON document found at a SpaceAPI endpoint." ;
    rdfs:isDefinedBy <http://www.spacerdf.org/schema.xml> ;
    rdfs:subClassOf foaf:Document .

:State
    a owl:Class ;
    rdfs:comment "The state of a hackerspace. The validity of instances of this class is time-limited." ;
    rdfs:isDefinedBy <http://www.spacerdf.org/schema.xml> .

:email
    a owl:ObjectProperty ;
    rdfs:comment "A contact email address for the hackerspace. If this address is a mailing list, consider using space:ml instead." ;
    rdfs:domain :Space ;
    rdfs:isDefinedBy <http://www.spacerdf.org/schema.xml> ;
    rdfs:subPropertyOf foaf:mbox .

:logo
    a owl:ObjectProperty ;
    rdfs:comment "A URL for the hackerspace's logo." ;
    rdfs:domain :Space ;
    rdfs:isDefinedBy <http://www.spacerdf.org/schema.xml> ;
    rdfs:range foaf:Image ;
    rdfs:subPropertyOf foaf:logo .

:ml
    a owl:ObjectProperty ;
    rdfs:comment "The primary mailing list for a hackerspace." ;
    rdfs:domain :Space ;
    rdfs:isDefinedBy <http://www.spacerdf.org/schema.xml> .

:name
    a owl:DatatypeProperty ;
    rdfs:comment "The name of the hackerspace." ;
    rdfs:domain :Space ;
    rdfs:isDefinedBy <http://www.spacerdf.org/schema.xml> ;
    rdfs:range xsd:string ;
    rdfs:subPropertyOf foaf:name .

:open
    a owl:DatatypeProperty ;
    rdfs:comment "Boolean value reflecting whether or not the space is open or closed for a given State." ;
    rdfs:domain :State ;
    rdfs:isDefinedBy <http://www.spacerdf.org/schema.xml> ;
    rdfs:range xsd:boolean .

:phone
    a owl:ObjectProperty ;
    rdfs:comment "Either a tel:, sip: or h323: URI for contacting the hackerspace with voice (and maybe video)." ;
    rdfs:domain :Space ;
    rdfs:isDefinedBy <http://www.spacerdf.org/schema.xml> ;
    rdfs:subPropertyOf foaf:phone .

:spaceAPI
    a owl:ObjectProperty ;
    rdfs:comment "A link to the SpaceAPI endpoint for a hackerspace." ;
    rdfs:domain :Space ;
    rdfs:isDefinedBy <http://www.spacerdf.org/schema.xml> ;
    rdfs:range :SpaceAPIDocument .

:triggerPerson
    a owl:ObjectProperty ;
    rdfs:comment "A foaf:PersonalProfileDocument for the person that triggered the State change." ;
    rdfs:domain :State ;
    rdfs:isDefinedBy <http://www.spacerdf.org/schema.xml> ;
    rdfs:range foaf:PersonalProfileDocument .

:triggeredBy
    a owl:DatatypeProperty ;
    rdfs:comment "The name, in the loosest sense of the word, of the person that triggered the State change." ;
    rdfs:domain :State ;
    rdfs:isDefinedBy <http://www.spacerdf.org/schema.xml> ;
    rdfs:range xsd:string .

:twitter
    a owl:ObjectProperty ;
    rdfs:comment "The Twitter account for a hackerspace." ;
    rdfs:domain :Space ;
    rdfs:isDefinedBy <http://www.spacerdf.org/schema.xml> ;
    rdfs:range foaf:OnlineAccount ;
    rdfs:subPropertyOf foaf:account .

:url
    a owl:ObjectProperty ;
    rdfs:comment "The URL of the hackerspace's homepage." ;
    rdfs:domain :Space ;
    rdfs:isDefinedBy <http://www.spacerdf.org/schema.xml> ;
    rdfs:range foaf:Document ;
    rdfs:subPropertyOf foaf:homepage .
